coq/model/Consistency2.v
@@ -4,174 +4,6 @@ From compcert.common Require Import Memory AST.
 From bpf.model Require Import ebpf rBPFCommType rBPFSyntax MyTactic.
 From bpf.model Require Import rBPFDecoder rBPFEncoder BitfieldLemma BinSolver.
 
-Lemma some_eq_eq: forall {A:Type} (a b:A),
-  Some a = Some b -> a = b.
-Proof.
-  intros.
-  inversion H.
-  reflexivity.
-Qed.
-
-Ltac simp_if_context_false :=
-  let K := fresh "K" in
-  match goal with
-    | H: (if ?A then _ else _) = _ |- _ => destruct A eqn: K; [ inversion H | simp_if_context_false]
-    | H: None = Some _ |- _ => inversion H
-    end.
-
-Ltac simp_if_context_post :=
-    match goal with
-    | K: (Z.to_nat ?v =? ?n)%nat = true |- Z.of_nat ?n = ?v  =>
-  rewrite Nat.eqb_eq in K;
-rewrite <- K;
-rewrite Z2Nat.id; [reflexivity | assumption]
-    end.
-
-Ltac simp_if_context :=
-  simp_if_context_false; simp_if_context_post.
-
-Lemma bpf_reg_decode_eq:
-  forall v r
-   (HZ: (0 <= v)%Z)
-    (HR: nat_to_bpf_ireg (Z.to_nat v) = Some r),
-    Z.of_nat (bpf_ireg_to_nat r) = v.
-Proof.
-  intros.
-  unfold nat_to_bpf_ireg, bpf_ireg_to_nat in *.
-  destruct r; simp_if_context.
-Qed.
-
-Lemma int64_unsigned_ge_0:
-  forall v,
-    0 <= Int64.unsigned v.
-Proof.
-  intros.
-  pose proof (Int64.unsigned_range_2 v) as H.
-  lia.
-Qed.
-
-Lemma int64_eq_iff:
-  forall x y,
-    Int64.eq x y = true <-> x = y.
-Proof.
-  intros.
-  split.
-  apply Int64.same_if_eq.
-  intro Heq; subst.
-  apply Int64.eq_true.
-Qed.
-
-Lemma int16_eq_iff:
-  forall x y,
-    Int16.eq x y = true <-> x = y.
-Proof.
-  intros.
-  split.
-  apply Int16.same_if_eq.
-  intro Heq; subst.
-  apply Int16.eq_true.
-Qed.
-
-Lemma byte_eq_iff:
-  forall x y,
-    Byte.eq x y = true <-> x = y.
-Proof.
-  intros.
-  split.
-  apply Byte.same_if_eq.
-  intro Heq; subst.
-  apply Byte.eq_true.
-Qed.
-
-
-Lemma int64_sign_int_extract_32_eq:
-  forall i,
-    (Int64.repr
-     (Int.unsigned
-        (Int.repr
-           (Int64.signed
-              (Int64.unsigned_bitfield_extract 32 32 i))))) = (Int64.unsigned_bitfield_extract 32 32 i).
-Proof.
-  intros.
-  unfold Int64.unsigned_bitfield_extract. simpl.
-  rewrite Int.unsigned_repr; [rewrite Int64.repr_signed; reflexivity |]. 
-  rewrite Int64.signed_eq_unsigned;
-  pose proof Int64.zero_ext_range 32 (Int64.shru i (Int64.repr 32)) as Hrange;
-  unfold Int64.zwordsize, two_p, two_power_pos in Hrange;
-  simpl in Hrange.
-  - change Int.max_unsigned with 4294967295.
-    lia.
-  - change Int64.max_signed with 9223372036854775807.
-    lia.
-Qed.
-
-
-Lemma int64_unsign_byte_extract_8_eq:
-  forall i,
-    (Int64.repr
-       (Byte.unsigned
-          (Byte.repr
-             (Int64.unsigned
-                (Int64.unsigned_bitfield_extract
-                   (Z.of_nat 0) 
-                   (Z.of_nat 8) i))))) =
-    (Int64.unsigned_bitfield_extract
-                             (Z.of_nat 0) 
-                             (Z.of_nat 8) i).
-Proof.
-  intros.
-  unfold Int64.unsigned_bitfield_extract. simpl.
-  rewrite Byte.unsigned_repr; [rewrite Int64.repr_unsigned; reflexivity |].
-  pose proof Int64.zero_ext_range 8 (Int64.shru i (Int64.repr 0)) as Hrange.
-  unfold Int64.zwordsize, two_p, two_power_pos in Hrange.
-  simpl in Hrange.
-  change Byte.max_unsigned with 255.
-  lia.
-Qed.
-
-
-Lemma int64_sign_int16_extract_16_eq:
-  forall i,
-    (Int64.repr
-        (Int16.unsigned
-           (Int16.repr
-              (Int64.signed
-                 (Int64.unsigned_bitfield_extract
-                    (Z.of_nat 16) (Z.of_nat 16) i))))) =
-    (Int64.unsigned_bitfield_extract
-                    (Z.of_nat 16) (Z.of_nat 16) i).
-Proof.
-  intros.
-  unfold Int64.unsigned_bitfield_extract.
-  rewrite Int16.unsigned_repr; [rewrite Int64.repr_signed; reflexivity |].
-  simpl.
-  rewrite Int64.signed_eq_unsigned;
-  pose proof Int64.zero_ext_range 16 (Int64.shru i (Int64.repr 16)) as Hrange;
-  unfold Int64.zwordsize, two_p, two_power_pos in Hrange;
-  simpl in Hrange.
-  - change Int16.max_unsigned with 65535.
-    lia.
-  - change Int64.max_signed with 9223372036854775807.
-    lia.
-Qed.
-
-Lemma int64_unsign_z_nat_16_eq :
-  forall i,
-    (Int64.repr
-           (Z.of_nat
-              (Z.to_nat
-                 (Int64.unsigned i)))) = i.
-Proof.
-  intros.
-  rewrite Z2Nat.id.
-  - rewrite Int64.repr_unsigned.
-    reflexivity.
-  - pose proof Int64.unsigned_range i as Hrange.
-    destruct Hrange as [H1 H2].
-    apply H1.
-Qed.
-
-
 Lemma rbpf_decode_encode_consistency:
   forall pc l ins
     (Hdecode: rbpf_decoder pc l = Some ins),
@@ -181,96 +13,700 @@ Proof.
   unfold rbpf_encoder, rbpf_decoder in *.
   intros.
   destruct nth_error eqn:Hnth; [| inversion Hdecode].
-  destruct ins; try ( eexists; split; [reflexivity |] ).
-  - (* LDDW*)
-    destruct (_ =? _)%Z eqn: Hlddw in Hdecode.
-    + destruct nth_error eqn:Hnth1 in Hdecode; [| inversion Hdecode].
-      destruct (nat_to_bpf_ireg _) as [dst | ] eqn: Hdst; [| inversion Hdecode].
-      destruct (_ && _)%bool eqn: Hlddwb in Hdecode; inversion Hdecode; subst.
+  eexists; split; [reflexivity |].
+  destruct (_ =? _)%Z eqn: Hlddw in Hdecode.
+  {(*          BPF_LD_IMM            *)
+    destruct nth_error eqn:Hnth1 in Hdecode; [| inversion Hdecode].
+    destruct (nat_to_bpf_ireg _) as [dst | ] eqn: Hdst; [| inversion Hdecode].
+    destruct (_ && _)%bool eqn: Hlddwb in Hdecode; inversion Hdecode; subst.
+    rewrite ! Bool.andb_true_iff in *.
+    destruct Hlddwb as (((((Hb1 & Hb2) & Hb3) & Hb4) & Hb5) & Hb6).
+    rewrite ! Nat.eqb_eq, Z.eqb_eq in *.
+    rewrite ! int16_eq_iff, byte_eq_iff in *.
+    rewrite <- Hb1 at 1.
+    rewrite <- Hb2 at 1.
+    rewrite <- Hb3 at 1.
+    rewrite <- Hb4 at 9.
+    rewrite <- Hb5 at 11.
+    rewrite <- Hb6 at 1.
+    rewrite <- Hlddw.
+    simpl in *.
+    rewrite Hnth, Hnth1.
+    unfold_bin.
+    erewrite bpf_reg_decode_eq with (r := dst); [| apply int64_unsigned_ge_0 | apply Hdst].
+    clear Hdecode Hnth Hnth1 Hlddw.
+    apply andb_true_intro.
+    split.
+    * apply int64_eq_iff.
+      rewrite ! Int64.repr_unsigned, Byte.repr_unsigned.
+      rewrite ! int64_sign_int_extract_32_eq, int64_sign_int16_extract_16_eq,  int64_unsign_byte_extract_8_eq, int64_unsign_z_nat_16_eq.
+      bsolver.
+    * apply andb_true_intro.
+      split; [| reflexivity].
+      apply int64_eq_iff.
+      rewrite ! int64_sign_int_extract_32_eq, int64_sign_int16_extract_16_eq,  int64_unsign_byte_extract_8_eq, int64_unsign_z_nat_16_eq, int64_unsign_z_nat_16_eq.
+      bsolver.
+  }
+  unfold rbpf_decoder_one in *.
+  destruct (_ =? _)%Z eqn: Hadd in Hdecode.
+  {
+    destruct (_ =? _)%nat eqn:Hdst in Hdecode.
+    { (*          BPF_ADD_STK            *)
+      destruct (_ && _)%bool eqn: Haddstk in Hdecode; inversion Hdecode. subst.
       rewrite ! Bool.andb_true_iff in *.
-      destruct Hlddwb as (((((Hb1 & Hb2) & Hb3) & Hb4) & Hb5) & Hb6).
-      rewrite ! Nat.eqb_eq, Z.eqb_eq in *.
-      rewrite ! int16_eq_iff, byte_eq_iff in *.
-      rewrite <- Hb1 at 1.
-      rewrite <- Hb2 at 1.
-      rewrite <- Hb3 at 1.
-      rewrite <- Hb4 at 9.
-      rewrite <- Hb5 at 11.
-      rewrite <- Hb6 at 1.
-      rewrite <- Hlddw.
+      destruct Haddstk as (Hb1 & Hb2).
+      rewrite ! Nat.eqb_eq, Z.eqb_eq, int16_eq_iff in *.
+      simpl in Hadd.
+      rewrite <- Hadd.
+      rewrite <- Hdst at 1.
+      rewrite <- Hb1 at 5.
+      unfold Int16.zero in Hb2.
+      rewrite <- Hb2.
       simpl in *.
-      rewrite Hnth, Hnth1.
+      rewrite Hnth.
       unfold_bin.
-      erewrite bpf_reg_decode_eq with (r := b); [| apply int64_unsigned_ge_0 | apply Hdst].
-      clear Hdecode Hnth Hnth1 Hlddw.
       apply andb_true_intro.
-      split.
-      * apply int64_eq_iff.
-        rewrite ! Int64.repr_unsigned, Byte.repr_unsigned.
-        rewrite ! int64_sign_int_extract_32_eq, int64_sign_int16_extract_16_eq,  int64_unsign_byte_extract_8_eq, int64_unsign_z_nat_16_eq.
-        bsolver.
-      * apply andb_true_intro.
-        split; [| reflexivity].
-        apply int64_eq_iff.
-        rewrite ! int64_sign_int_extract_32_eq, int64_sign_int16_extract_16_eq,  int64_unsign_byte_extract_8_eq, int64_unsign_z_nat_16_eq, int64_unsign_z_nat_16_eq.
-        bsolver.
-    + exfalso.
-      clear Hlddw Hnth.
-      unfold rbpf_decoder_one, binary_to_int64, decode_bpf, encode_bpf in Hdecode.
+      split; [| reflexivity].
+      apply int64_eq_iff.
+      rewrite Z2Nat.id; [| apply int64_unsigned_ge_0].
+      rewrite ! Byte.repr_unsigned, Int64.repr_unsigned.
+      rewrite ! int64_sign_int_extract_32_eq, int64_sign_int16_extract_16_eq,  int64_unsign_byte_extract_8_eq, int64_unsign_z_nat_16_eq.
+      bsolver.
+    }(*          BPF_ADD           *)
+    destruct (_ && _)%bool eqn: Haddnum in Hdecode; [| inversion Hdecode].
+    rewrite ! Bool.andb_true_iff in *.
+    destruct Haddnum as (Hb1 & Hb2).
+    rewrite ! Nat.eqb_eq, Z.eqb_eq, int16_eq_iff in *.
+    simpl in Hadd.
+    clear Hlddw Hdst.
+    destruct (nat_to_bpf_ireg _) as [dst | ] eqn: Hdst; [| inversion Hdecode].
+    inversion Hdecode; subst.
+    rewrite <- Hadd.
+    rewrite <- Hb1 at 3.
+    unfold Int16.zero in Hb2.
+    rewrite <- Hb2.
+    simpl in *.
+    rewrite Hnth.
+    unfold_bin.
+    erewrite bpf_reg_decode_eq with (r := dst); [| apply int64_unsigned_ge_0 | apply Hdst].
+    apply andb_true_intro.
+    split; [| reflexivity].
+    apply int64_eq_iff.
+    rewrite Z2Nat.id; [| apply int64_unsigned_ge_0].
+    rewrite ! Byte.repr_unsigned, Int64.repr_unsigned, Int64.repr_unsigned.
+    rewrite ! int64_sign_int_extract_32_eq, int64_sign_int16_extract_16_eq,  int64_unsign_byte_extract_8_eq.
+    bsolver.
+  }
+  clear Hlddw Hadd.
+  destruct (nat_to_bpf_ireg _) as [dst | ] eqn: Hdst in Hdecode; [| inversion Hdecode].
+  destruct (nat_to_bpf_ireg _) as [src | ] eqn: Hsrc in Hdecode; [| inversion Hdecode].
+  do 4 ((*          BPF_LDX           *)
+    destruct (_ =? _)%Z eqn: Hldx in Hdecode;
+    try (
+      destruct (Int.eq _ _) eqn:Himm; [| inversion Hdecode];
+      inversion Hdecode; subst;
+      rewrite ! int_eq_iff, Z.eqb_eq in *;
+      simpl in Hldx;
+      unfold Int.zero in Himm;
+      rewrite <- Hldx;
+      rewrite <- Himm;
+      simpl in *;
+      rewrite Hnth;
+      unfold_bin;
+      erewrite bpf_reg_decode_eq with (r := dst); [| apply int64_unsigned_ge_0 | apply Hdst];
+      erewrite bpf_reg_decode_eq with (r := src); [| apply int64_unsigned_ge_0 | apply Hsrc];
+      apply andb_true_intro;
+      split; [| reflexivity];
+      apply int64_eq_iff;
+      rewrite ! Byte.repr_unsigned, Int64.repr_unsigned, Int64.repr_unsigned;
+      rewrite ! int64_sign_int_extract_32_eq, int64_sign_int16_extract_16_eq,  int64_unsign_byte_extract_8_eq;
+      bsolver
+    );
+    clear Hldx
+  ).
+  do 4 ((*          BPF_ST_IMM           *)
+    destruct (_ =? _)%Z eqn: Hst in Hdecode;
+    try (
+      destruct (_ =? _)%nat eqn:Himm; [| inversion Hdecode];
+      inversion Hdecode; subst;
+      rewrite ! Nat.eqb_eq, Z.eqb_eq in *;
+      simpl in Hst;
+      unfold Int.zero in Himm;
+      rewrite <- Hst at 1;
+      rewrite <- Himm at 3;
+      simpl in *;
+      rewrite Hnth;
+      unfold_bin;
+      erewrite bpf_reg_decode_eq with (r := dst); [| apply int64_unsigned_ge_0 | apply Hdst];
+      apply andb_true_intro;
+      split; [| reflexivity];
+      apply int64_eq_iff;
+      rewrite Z2Nat.id; [| apply int64_unsigned_ge_0];
+      rewrite ! Byte.repr_unsigned, Int64.repr_unsigned, Int64.repr_unsigned;
+      rewrite ! int64_sign_int_extract_32_eq, int64_sign_int16_extract_16_eq,  int64_unsign_byte_extract_8_eq;
+      bsolver
+    );
+    clear Hst
+  ).
+  do 4 ((*          BPF_ST_REG           *)
+    destruct (_ =? _)%Z eqn: Hst in Hdecode;
+    try (
+      destruct (Int.eq _ _)%nat eqn:Himm; [| inversion Hdecode];
+      inversion Hdecode; subst;
+      rewrite ! int_eq_iff, Z.eqb_eq in *;
+      simpl in Hst;
+      unfold Int.zero in Himm;
+      rewrite <- Hst at 1;
+      rewrite <- Himm;
+      simpl in *;
+      rewrite Hnth;
+      unfold_bin;
+      erewrite bpf_reg_decode_eq with (r := dst); [| apply int64_unsigned_ge_0 | apply Hdst];
+      erewrite bpf_reg_decode_eq with (r := src); [| apply int64_unsigned_ge_0 | apply Hsrc];
+      apply andb_true_intro;
+      split; [| reflexivity];
+      apply int64_eq_iff;
+      rewrite ! Byte.repr_unsigned, Int64.repr_unsigned, Int64.repr_unsigned;
+      rewrite ! int64_sign_int_extract_32_eq, int64_sign_int16_extract_16_eq,  int64_unsign_byte_extract_8_eq;
+      bsolver
+    );
+    clear Hst
+  ).
+  do 8 ((*          BPF_ALU           *)
+    destruct (_ =? _)%Z eqn: Halu in Hdecode;
+    try(
+        destruct (_ && _)%bool eqn:Halu2 in Hdecode; [| inversion Hdecode];
+        rewrite ! Bool.andb_true_iff in *;
+        destruct Halu2 as (Hb1 & Hb2);
+        rewrite ! Nat.eqb_eq, Z.eqb_eq, int16_eq_iff in *;
+        inversion Hdecode; subst;
+        simpl in Halu;
+        unfold Int16.zero in Hb2;
+        rewrite <- Halu at 1;
+        rewrite <- Hb1 at 3;
+        rewrite <- Hb2;
+        simpl in *;
+        rewrite Hnth;
+        unfold_bin;
+        erewrite bpf_reg_decode_eq with (r := dst); [| apply int64_unsigned_ge_0 | apply Hdst];
+        apply andb_true_intro;
+        split; [| reflexivity];
+        apply int64_eq_iff;
+        rewrite Z2Nat.id; [| apply int64_unsigned_ge_0];
+        rewrite ! Byte.repr_unsigned, Int64.repr_unsigned, Int64.repr_unsigned;
+        rewrite ! int64_sign_int_extract_32_eq, int64_sign_int16_extract_16_eq,  int64_unsign_byte_extract_8_eq;
+        bsolver
+    );
+    clear Halu;
+    destruct (_ =? _)%Z eqn: Halu in Hdecode;
+    try(
+      destruct (_ && _)%bool eqn:Halu2 in Hdecode; [| inversion Hdecode];
+      rewrite ! Bool.andb_true_iff in *;
+      destruct Halu2 as (Hb1 & Hb2);
+      rewrite ! int_eq_iff, Z.eqb_eq, int16_eq_iff in *;
+      inversion Hdecode; subst;
+      simpl in Halu;
+      unfold Int16.zero in Hb2;
+      unfold Int.zero in Hb1;
+      rewrite <- Halu at 1;
+      rewrite <- Hb1;
+      rewrite <- Hb2;
+      simpl in *;
+      rewrite Hnth;
+      unfold_bin;
+      erewrite bpf_reg_decode_eq with (r := dst); [| apply int64_unsigned_ge_0 | apply Hdst];
+      erewrite bpf_reg_decode_eq with (r := src); [| apply int64_unsigned_ge_0 | apply Hsrc];
+      apply andb_true_intro;
+      split; [| reflexivity];
+      apply int64_eq_iff;
+      rewrite ! Byte.repr_unsigned, Int64.repr_unsigned, Int64.repr_unsigned;
+      rewrite ! int64_sign_int_extract_32_eq, int64_sign_int16_extract_16_eq,  int64_unsign_byte_extract_8_eq;
+      bsolver
+    );
+    clear Halu
+  ).
+
+  destruct (_ =? _)%Z eqn: Hneg32 in Hdecode.
+  {  (*          BPF_NEG32           *)
+    destruct (_ && _)%bool eqn:Hneg322 in Hdecode; [| inversion Hdecode].
+    rewrite ! Bool.andb_true_iff in *.
+    destruct Hneg322 as ((Hb1 & Hb2) & Hb3).
+    rewrite ! Nat.eqb_eq, Z.eqb_eq, int16_eq_iff, int_eq_iff in *.
+    inversion Hdecode; subst.
+    simpl in Hneg32.
+    rewrite <- Hneg32.
+    rewrite <- Hb1 at 3.
+    unfold Int16.zero in Hb2.
+    unfold Int.zero in Hb3.
+    rewrite <- Hb2.
+    rewrite <- Hb3.
+    simpl in *.
+    rewrite Hnth.
+    unfold_bin.
+    erewrite bpf_reg_decode_eq with (r := dst); [| apply int64_unsigned_ge_0 | apply Hdst].
+    apply andb_true_intro.
+    split; [| reflexivity].
+    apply int64_eq_iff.
+    rewrite Z2Nat.id; [| apply int64_unsigned_ge_0].
+    rewrite ! Byte.repr_unsigned, Int64.repr_unsigned, Int64.repr_unsigned.
+    rewrite ! int64_sign_int_extract_32_eq, int64_sign_int16_extract_16_eq,  int64_unsign_byte_extract_8_eq.
+    bsolver.
+  }
+  clear Hneg32.
+  do 4 ((*          BPF_ALU           *)
+    destruct (_ =? _)%Z eqn: Halu in Hdecode;
+    try(
+        destruct (_ && _)%bool eqn:Halu2 in Hdecode; [| inversion Hdecode];
+        rewrite ! Bool.andb_true_iff in *;
+        destruct Halu2 as (Hb1 & Hb2);
+        rewrite ! Nat.eqb_eq, Z.eqb_eq, int16_eq_iff in *;
+        inversion Hdecode; subst;
+        simpl in Halu;
+        unfold Int16.zero in Hb2;
+        rewrite <- Halu at 1;
+        rewrite <- Hb1 at 3;
+        rewrite <- Hb2;
+        simpl in *;
+        rewrite Hnth;
+        unfold_bin;
+        erewrite bpf_reg_decode_eq with (r := dst); [| apply int64_unsigned_ge_0 | apply Hdst];
+        apply andb_true_intro;
+        split; [| reflexivity];
+        apply int64_eq_iff;
+        rewrite Z2Nat.id; [| apply int64_unsigned_ge_0];
+        rewrite ! Byte.repr_unsigned, Int64.repr_unsigned, Int64.repr_unsigned;
+        rewrite ! int64_sign_int_extract_32_eq, int64_sign_int16_extract_16_eq,  int64_unsign_byte_extract_8_eq;
+        bsolver
+    );
+    clear Halu;
+    destruct (_ =? _)%Z eqn: Halu in Hdecode;
+    try(
+      destruct (_ && _)%bool eqn:Halu2 in Hdecode; [| inversion Hdecode];
+      rewrite ! Bool.andb_true_iff in *;
+      destruct Halu2 as (Hb1 & Hb2);
+      rewrite ! int_eq_iff, Z.eqb_eq, int16_eq_iff in *;
+      inversion Hdecode; subst;
+      simpl in Halu;
+      unfold Int16.zero in Hb2;
+      unfold Int.zero in Hb1;
+      rewrite <- Halu at 1;
+      rewrite <- Hb1;
+      rewrite <- Hb2;
+      simpl in *;
+      rewrite Hnth;
+      unfold_bin;
+      erewrite bpf_reg_decode_eq with (r := dst); [| apply int64_unsigned_ge_0 | apply Hdst];
+      erewrite bpf_reg_decode_eq with (r := src); [| apply int64_unsigned_ge_0 | apply Hsrc];
+      apply andb_true_intro;
+      split; [| reflexivity];
+      apply int64_eq_iff;
+      rewrite ! Byte.repr_unsigned, Int64.repr_unsigned, Int64.repr_unsigned;
+      rewrite ! int64_sign_int_extract_32_eq, int64_sign_int16_extract_16_eq,  int64_unsign_byte_extract_8_eq;
+      bsolver
+    );
+    clear Halu
+  ).
+  do 2 ((*          BPF_BE/LE           *)
+    destruct (_ =? _)%Z eqn: Hswap in Hdecode;
+    try(
+      destruct (_ && _)%bool eqn:Hswap2 in Hdecode; [| inversion Hdecode];
+      rewrite ! Bool.andb_true_iff in *;
+      destruct Hswap2 as (Hb1 & Hb2);
+      rewrite ! Nat.eqb_eq, Z.eqb_eq, int16_eq_iff in *;
+      inversion Hdecode; subst;
+      simpl in Hswap;
+      unfold Int16.zero in Hb2;
+      rewrite <- Hswap at 1;
+      rewrite <- Hb1 at 3;
+      rewrite <- Hb2;
+      simpl in *;
+      rewrite Hnth;
+      unfold_bin;
+      erewrite bpf_reg_decode_eq with (r := dst); [| apply int64_unsigned_ge_0 | apply Hdst];
+      apply andb_true_intro;
+      split; [| reflexivity];
+      apply int64_eq_iff;
+      rewrite Z2Nat.id; [| apply int64_unsigned_ge_0];
+      rewrite ! Byte.repr_unsigned, Int64.repr_unsigned, Int64.repr_unsigned;
+      rewrite ! int64_sign_int_extract_32_eq, int64_sign_int16_extract_16_eq,  int64_unsign_byte_extract_8_eq;
+      bsolver
+    );
+    clear Hswap
+  ).
+
+  destruct (_ =? _)%Z eqn: Halu64 in Hdecode.
+  {(*          BPF_ALU64           *)
+    destruct (_ && _)%bool eqn:Halu642 in Hdecode; [| inversion Hdecode].
+      rewrite ! Bool.andb_true_iff in *.
+      destruct Halu642 as (Hb1 & Hb2).
+      rewrite ! int_eq_iff, Z.eqb_eq, int16_eq_iff in *.
+      inversion Hdecode; subst.
+      simpl in Halu64.
+      unfold Int16.zero in Hb2.
+      unfold Int.zero in Hb1.
+      rewrite <- Halu64 at 1.
+      rewrite <- Hb1.
+      rewrite <- Hb2.
       simpl in *.
-      destruct (_ =? _)%Z eqn:Heq1 in Hdecode.
-      * destruct (_ =? _)%nat eqn:Hstk in Hdecode; [inversion Hdecode |].
-        destruct (nat_to_bpf_ireg (Z.to_nat (Int64.unsigned (Int64.unsigned_bitfield_extract 8 4 i)))) eqn:Hnat in Hdecode;
-        inversion Hdecode.
-      * repeat (destruct (nat_to_bpf_ireg _) in Hdecode; [| inversion Hdecode]).
-        repeat (destruct (_ =? _) in Hdecode; [inversion Hdecode |]).
-        inversion Hdecode.
-  - destruct (_ =? _)%Z eqn: Hlddw in Hdecode.
-    + destruct nth_error eqn:Hnth1 in Hdecode; [| inversion Hdecode].
-      destruct (nat_to_bpf_ireg _) as [dst | ] eqn: Hdst; [| inversion Hdecode].
-      destruct (_ && _)%bool eqn: Hlddwb in Hdecode; inversion Hdecode.
-    + unfold rbpf_decoder_one, binary_to_int64, decode_bpf, encode_bpf in *.
+      rewrite Hnth.
+      unfold_bin.
+      erewrite bpf_reg_decode_eq with (r := dst); [| apply int64_unsigned_ge_0 | apply Hdst].
+      erewrite bpf_reg_decode_eq with (r := src); [| apply int64_unsigned_ge_0 | apply Hsrc].
+      apply andb_true_intro.
+      split; [| reflexivity].
+      apply int64_eq_iff.
+      rewrite ! Byte.repr_unsigned, Int64.repr_unsigned, Int64.repr_unsigned.
+      rewrite ! int64_sign_int_extract_32_eq, int64_sign_int16_extract_16_eq,  int64_unsign_byte_extract_8_eq.
+      bsolver.
+  }
+  clear Halu64.
+  do 7 ((*          BPF_ALU64           *)
+    destruct (_ =? _)%Z eqn: Halu64 in Hdecode;
+    try(
+        destruct (_ && _)%bool eqn:Halu642 in Hdecode; [| inversion Hdecode];
+        rewrite ! Bool.andb_true_iff in *;
+        destruct Halu642 as (Hb1 & Hb2);
+        rewrite ! Nat.eqb_eq, Z.eqb_eq, int16_eq_iff in *;
+        inversion Hdecode; subst;
+        simpl in Halu64;
+        unfold Int16.zero in Hb2;
+        rewrite <- Halu64 at 1;
+        rewrite <- Hb1 at 3;
+        rewrite <- Hb2;
+        simpl in *;
+        rewrite Hnth;
+        unfold_bin;
+        erewrite bpf_reg_decode_eq with (r := dst); [| apply int64_unsigned_ge_0 | apply Hdst];
+        apply andb_true_intro;
+        split; [| reflexivity];
+        apply int64_eq_iff;
+        rewrite Z2Nat.id; [| apply int64_unsigned_ge_0];
+        rewrite ! Byte.repr_unsigned, Int64.repr_unsigned, Int64.repr_unsigned;
+        rewrite ! int64_sign_int_extract_32_eq, int64_sign_int16_extract_16_eq,  int64_unsign_byte_extract_8_eq;
+        bsolver
+    );
+    clear Halu64;
+    destruct (_ =? _)%Z eqn: Halu64 in Hdecode;
+    try(
+      destruct (_ && _)%bool eqn:Halu642 in Hdecode; [| inversion Hdecode];
+      rewrite ! Bool.andb_true_iff in *;
+      destruct Halu642 as (Hb1 & Hb2);
+      rewrite ! int_eq_iff, Z.eqb_eq, int16_eq_iff in *;
+      inversion Hdecode; subst;
+      simpl in Halu64;
+      unfold Int16.zero in Hb2;
+      unfold Int.zero in Hb1;
+      rewrite <- Halu64 at 1;
+      rewrite <- Hb1;
+      rewrite <- Hb2;
+      simpl in *;
+      rewrite Hnth;
+      unfold_bin;
+      erewrite bpf_reg_decode_eq with (r := dst); [| apply int64_unsigned_ge_0 | apply Hdst];
+      erewrite bpf_reg_decode_eq with (r := src); [| apply int64_unsigned_ge_0 | apply Hsrc];
+      apply andb_true_intro;
+      split; [| reflexivity];
+      apply int64_eq_iff;
+      rewrite ! Byte.repr_unsigned, Int64.repr_unsigned, Int64.repr_unsigned;
+      rewrite ! int64_sign_int_extract_32_eq, int64_sign_int16_extract_16_eq,  int64_unsign_byte_extract_8_eq;
+      bsolver
+    );
+    clear Halu64
+  ).
+  destruct (_ =? _)%Z eqn: Hneg64 in Hdecode.
+  {(*          BPF_NEG64           *)
+    destruct (_ && _)%bool eqn:Hneg642 in Hdecode; [| inversion Hdecode].
+    rewrite ! Bool.andb_true_iff in *.
+    destruct Hneg642 as ((Hb1 & Hb2) & Hb3).
+    rewrite ! Nat.eqb_eq, int16_eq_iff, int_eq_iff, Z.eqb_eq in *.
+    inversion Hdecode; subst.
+    simpl in Hneg64.
+    rewrite <- Hneg64.
+    rewrite <- Hb1 at 3.
+    unfold Int16.zero in Hb2.
+    unfold Int.zero in Hb3.
+    rewrite <- Hb2.
+    rewrite <- Hb3.
+    simpl in *.
+    rewrite Hnth.
+    unfold_bin.
+    erewrite bpf_reg_decode_eq with (r := dst); [| apply int64_unsigned_ge_0 | apply Hdst].
+    apply andb_true_intro.
+    split; [| reflexivity].
+    apply int64_eq_iff.
+    rewrite Z2Nat.id; [| apply int64_unsigned_ge_0].
+    rewrite ! Byte.repr_unsigned, Int64.repr_unsigned, Int64.repr_unsigned.
+    rewrite ! int64_sign_int_extract_32_eq, int64_sign_int16_extract_16_eq,  int64_unsign_byte_extract_8_eq.
+    bsolver.
+  }
+  clear Hneg64.
+  do 4 ((*          BPF_ALU64           *)
+    destruct (_ =? _)%Z eqn: Halu64 in Hdecode;
+    try(
+        destruct (_ && _)%bool eqn:Halu642 in Hdecode; [| inversion Hdecode];
+        rewrite ! Bool.andb_true_iff in *;
+        destruct Halu642 as (Hb1 & Hb2);
+        rewrite ! Nat.eqb_eq, Z.eqb_eq, int16_eq_iff in *;
+        inversion Hdecode; subst;
+        simpl in Halu64;
+        unfold Int16.zero in Hb2;
+        rewrite <- Halu64 at 1;
+        rewrite <- Hb1 at 3;
+        rewrite <- Hb2;
+        simpl in *;
+        rewrite Hnth;
+        unfold_bin;
+        erewrite bpf_reg_decode_eq with (r := dst); [| apply int64_unsigned_ge_0 | apply Hdst];
+        apply andb_true_intro;
+        split; [| reflexivity];
+        apply int64_eq_iff;
+        rewrite Z2Nat.id; [| apply int64_unsigned_ge_0];
+        rewrite ! Byte.repr_unsigned, Int64.repr_unsigned, Int64.repr_unsigned;
+        rewrite ! int64_sign_int_extract_32_eq, int64_sign_int16_extract_16_eq,  int64_unsign_byte_extract_8_eq;
+        bsolver
+    );
+    clear Halu64;
+    destruct (_ =? _)%Z eqn: Halu64 in Hdecode;
+    try(
+      destruct (_ && _)%bool eqn:Halu642 in Hdecode; [| inversion Hdecode];
+      rewrite ! Bool.andb_true_iff in *;
+      destruct Halu642 as (Hb1 & Hb2);
+      rewrite ! int_eq_iff, Z.eqb_eq, int16_eq_iff in *;
+      inversion Hdecode; subst;
+      simpl in Halu64;
+      unfold Int16.zero in Hb2;
+      unfold Int.zero in Hb1;
+      rewrite <- Halu64 at 1;
+      rewrite <- Hb1;
+      rewrite <- Hb2;
+      simpl in *;
+      rewrite Hnth;
+      unfold_bin;
+      erewrite bpf_reg_decode_eq with (r := dst); [| apply int64_unsigned_ge_0 | apply Hdst];
+      erewrite bpf_reg_decode_eq with (r := src); [| apply int64_unsigned_ge_0 | apply Hsrc];
+      apply andb_true_intro;
+      split; [| reflexivity];
+      apply int64_eq_iff;
+      rewrite ! Byte.repr_unsigned, Int64.repr_unsigned, Int64.repr_unsigned;
+      rewrite ! int64_sign_int_extract_32_eq, int64_sign_int16_extract_16_eq,  int64_unsign_byte_extract_8_eq;
+      bsolver
+    );
+    clear Halu64
+  ).
+  destruct (_ =? _)%Z eqn: Hhor64 in Hdecode.
+  {(*          BPF_HOR64_IMM           *)
+    destruct (_ && _)%bool eqn:Hhor642 in Hdecode; [| inversion Hdecode].
+    rewrite ! Bool.andb_true_iff in *.
+    destruct Hhor642 as (Hb1 & Hb2).
+    rewrite ! Nat.eqb_eq, Z.eqb_eq, int16_eq_iff in *.
+    inversion Hdecode; subst.
+    simpl in Hhor64.
+    unfold Int16.zero in Hb2.
+    rewrite <- Hhor64 at 1.
+    rewrite <- Hb1 at 3.
+    rewrite <- Hb2.
+    simpl in *.
+    rewrite Hnth.
+    unfold_bin.
+    erewrite bpf_reg_decode_eq with (r := dst); [| apply int64_unsigned_ge_0 | apply Hdst].
+    apply andb_true_intro.
+    split; [| reflexivity].
+    apply int64_eq_iff.
+    rewrite Z2Nat.id; [| apply int64_unsigned_ge_0].
+    rewrite ! Byte.repr_unsigned, Int64.repr_unsigned, Int64.repr_unsigned.
+    rewrite ! int64_sign_int_extract_32_eq, int64_sign_int16_extract_16_eq,  int64_unsign_byte_extract_8_eq.
+    bsolver.
+  }
+  clear Hhor64.
+  do 12 ((*          BPF_PQR           *)
+    destruct (_ =? _)%Z eqn: Hpqr in Hdecode;
+    try(
+        destruct (_ && _)%bool eqn:Hpqr2 in Hdecode; [| inversion Hdecode];
+        rewrite ! Bool.andb_true_iff in *;
+        destruct Hpqr2 as (Hb1 & Hb2);
+        rewrite ! Nat.eqb_eq, Z.eqb_eq, int16_eq_iff in *;
+        inversion Hdecode; subst;
+        simpl in Hpqr;
+        unfold Int16.zero in Hb2;
+        rewrite <- Hpqr at 1;
+        rewrite <- Hb1 at 3;
+        rewrite <- Hb2;
+        simpl in *;
+        rewrite Hnth;
+        unfold_bin;
+        erewrite bpf_reg_decode_eq with (r := dst); [| apply int64_unsigned_ge_0 | apply Hdst];
+        apply andb_true_intro;
+        split; [| reflexivity];
+        apply int64_eq_iff;
+        rewrite Z2Nat.id; [| apply int64_unsigned_ge_0];
+        rewrite ! Byte.repr_unsigned, Int64.repr_unsigned, Int64.repr_unsigned;
+        rewrite ! int64_sign_int_extract_32_eq, int64_sign_int16_extract_16_eq,  int64_unsign_byte_extract_8_eq;
+        bsolver
+    );
+    clear Hpqr;
+    destruct (_ =? _)%Z eqn: Hpqr in Hdecode;
+    try(
+      destruct (_ && _)%bool eqn:Hpqr2 in Hdecode; [| inversion Hdecode];
+      rewrite ! Bool.andb_true_iff in *;
+      destruct Hpqr2 as (Hb1 & Hb2);
+      rewrite ! int_eq_iff, Z.eqb_eq, int16_eq_iff in *;
+      inversion Hdecode; subst;
+      simpl in Hpqr;
+      unfold Int16.zero in Hb2;
+      unfold Int.zero in Hb1;
+      rewrite <- Hpqr at 1;
+      rewrite <- Hb1;
+      rewrite <- Hb2;
+      simpl in *;
+      rewrite Hnth;
+      unfold_bin;
+      erewrite bpf_reg_decode_eq with (r := dst); [| apply int64_unsigned_ge_0 | apply Hdst];
+      erewrite bpf_reg_decode_eq with (r := src); [| apply int64_unsigned_ge_0 | apply Hsrc];
+      apply andb_true_intro;
+      split; [| reflexivity];
+      apply int64_eq_iff;
+      rewrite ! Byte.repr_unsigned, Int64.repr_unsigned, Int64.repr_unsigned;
+      rewrite ! int64_sign_int_extract_32_eq, int64_sign_int16_extract_16_eq,  int64_unsign_byte_extract_8_eq;
+      bsolver
+    );
+    clear Hpqr
+  ).
+  destruct (_ =? _)%Z eqn: Hja in Hdecode.
+  {(*          BPF_JA           *)
+      destruct (_ && _)%bool eqn:Hja2 in Hdecode; [| inversion Hdecode].
+      rewrite ! Bool.andb_true_iff in *.
+      destruct Hja2 as ((Hb1 & Hb2) & Hb3).
+      rewrite ! int_eq_iff, Z.eqb_eq, Nat.eqb_eq in *.
+      inversion Hdecode; subst.
+      simpl in Hja.
+      unfold Int16.zero in Hb2.
+      unfold Int.zero in Hb3.
+      rewrite <- Hja at 1.
+      rewrite <- Hb1 at 4.
+      rewrite <- Hb2 at 3.
+      rewrite <- Hb3.
       simpl in *.
-      clear Hlddw.
-      destruct (_ =? _)%Z eqn:Heq1 in Hdecode.
-      * destruct (_ =? _)%nat eqn:Hstk in Hdecode; [inversion Hdecode |].
-        destruct (nat_to_bpf_ireg (Z.to_nat (Int64.unsigned (Int64.unsigned_bitfield_extract 8 4 i)))) eqn:Hnat in Hdecode;
-        inversion Hdecode.
-      * destruct (nat_to_bpf_ireg _) eqn:Hdst in Hdecode; [| inversion Hdecode].
-        destruct (nat_to_bpf_ireg _) eqn:Hsrc in Hdecode; [| inversion Hdecode].
-        destruct m.
-        destruct (_ =? _) eqn:Heq in Hdecode.
-        -- inversion Hdecode.
-           subst.
-           rewrite Hnth.
-           apply andb_true_intro.
-           split.
-           --- apply int64_eq_iff.
-               rewrite ! Byte.unsigned_repr in *; try (unfold Byte.max_unsigned; simpl; lia).
-               rewrite Z.eqb_eq in Heq.
-               rewrite <- Heq.
-               
-               bsolver.
-               Search Int64.bitfield_insert.
-               rewrite Z.eqb_neq in *.
-               admit.
+      rewrite Hnth.
+      unfold_bin.
+      apply andb_true_intro.
+      split; [| reflexivity].
+      apply int64_eq_iff.
+      rewrite Z2Nat.id; [| apply int64_unsigned_ge_0].
+      rewrite Z2Nat.id; [| apply int64_unsigned_ge_0].
+      rewrite ! Byte.repr_unsigned, Int64.repr_unsigned, Int64.repr_unsigned.
+      rewrite ! int64_sign_int_extract_32_eq, int64_sign_int16_extract_16_eq,  int64_unsign_byte_extract_8_eq.
+      bsolver.
+  }
+  clear Hja.
+  do 11 ((*          BPF_JUMP           *)
+    destruct (_ =? _)%Z eqn: Hjump in Hdecode;
+    try (
+      destruct (_ =? _)%nat eqn:Hsrc2; [| inversion Hdecode];
+      inversion Hdecode; subst;
+      rewrite ! Z.eqb_eq, Nat.eqb_eq in *;
+      simpl in Hjump;
+      unfold Int.zero in Hsrc2;
+      rewrite <- Hjump;
+      rewrite <- Hsrc2 at 3;
+      simpl in *;
+      rewrite Hnth;
+      unfold_bin;
+      erewrite bpf_reg_decode_eq with (r := dst); [| apply int64_unsigned_ge_0 | apply Hdst];
+      apply andb_true_intro;
+      split; [| reflexivity];
+      apply int64_eq_iff;
+      rewrite Z2Nat.id; [| apply int64_unsigned_ge_0];
+      rewrite ! Byte.repr_unsigned, Int64.repr_unsigned, Int64.repr_unsigned;
+      rewrite ! int64_sign_int_extract_32_eq, int64_sign_int16_extract_16_eq,  int64_unsign_byte_extract_8_eq;
+      bsolver
+    );
+    clear Hjump;
+    destruct (_ =? _)%Z eqn: Hjump in Hdecode;
+    try(
+      destruct (Int.eq _ _)%nat eqn:Himm; [| inversion Hdecode];
+      inversion Hdecode; subst;
+      rewrite ! Z.eqb_eq, int_eq_iff in *;
+      simpl in Hjump;
+      unfold Int.zero in Himm;
+      rewrite <- Hjump;
+      rewrite <- Himm;
+      simpl in *;
+      rewrite Hnth;
+      unfold_bin;
+      erewrite bpf_reg_decode_eq with (r := dst); [| apply int64_unsigned_ge_0 | apply Hdst];
+      erewrite bpf_reg_decode_eq with (r := src); [| apply int64_unsigned_ge_0 | apply Hsrc];
+      apply andb_true_intro;
+      split; [| reflexivity];
+      apply int64_eq_iff;
+      rewrite ! Byte.repr_unsigned, Int64.repr_unsigned, Int64.repr_unsigned;
+      rewrite ! int64_sign_int_extract_32_eq, int64_sign_int16_extract_16_eq,  int64_unsign_byte_extract_8_eq;
+      bsolver
+    );
+    clear Hjump
+  ).
+  do 2 ((*          BPF_CALL           *)
+    destruct (_ =? _)%Z eqn: Hcall in Hdecode;
+    try(
+      destruct (_ && _)%bool eqn:Hcall2 in Hdecode; [| inversion Hdecode];
+      rewrite ! Bool.andb_true_iff in *;
+      destruct Hcall2 as (Hb1 & Hb2);
+      rewrite ! int16_eq_iff, Z.eqb_eq, Nat.eqb_eq in *;
+      inversion Hdecode; subst;
+      simpl in Hcall;
+      unfold Int16.zero in Hb2;
+      rewrite <- Hcall;
+      rewrite <- Hb1 at 3;
+      rewrite <- Hb2;
+      simpl in *;
+      rewrite Hnth;
+      unfold_bin;
+      erewrite bpf_reg_decode_eq with (r := src); [| apply int64_unsigned_ge_0 | apply Hsrc];
+      apply andb_true_intro;
+      split; [| reflexivity];
+      apply int64_eq_iff;
+      rewrite Z2Nat.id; [| apply int64_unsigned_ge_0];
+      rewrite ! Byte.repr_unsigned, Int64.repr_unsigned, Int64.repr_unsigned;
+      rewrite ! int64_sign_int_extract_32_eq, int64_sign_int16_extract_16_eq,  int64_unsign_byte_extract_8_eq;
+      bsolver
+    );
+    clear Hcall
+  ).
+  destruct (_ =? _)%Z eqn: Hexit in Hdecode.
+  {
+    destruct (_ && _)%bool eqn:Hexit2 in Hdecode; [| inversion Hdecode].
+    rewrite ! Bool.andb_true_iff in *.
+    destruct Hexit2 as (((Hb1 & Hb2) & Hb3) & Hb4).
+    rewrite ! int_eq_iff, int16_eq_iff, Z.eqb_eq, Nat.eqb_eq in *.
+    inversion Hdecode; subst.
+    simpl in Hexit.
+    unfold Int16.zero in Hb2.
+    unfold Int.zero in Hb4.
+    rewrite <- Hexit.
+    rewrite <- Hb1 at 4.
+    rewrite <- Hb2.
+    rewrite <- Hb4.
+    rewrite <- Hb3 at 3.
+    simpl in *.
+    rewrite Hnth.
+    unfold_bin.
+    apply andb_true_intro.
+    split; [| reflexivity].
+    apply int64_eq_iff.
+    rewrite Z2Nat.id; [| apply int64_unsigned_ge_0].
+    rewrite Z2Nat.id; [| apply int64_unsigned_ge_0].
+    rewrite ! Byte.repr_unsigned, Int64.repr_unsigned, Int64.repr_unsigned.
+    rewrite ! int64_sign_int_extract_32_eq, int64_sign_int16_extract_16_eq,  int64_unsign_byte_extract_8_eq.
+    bsolver.
+  }
+  inversion Hdecode.
+Qed.
 
 
 
-        rewrite Hnth.
-        -- apply andb_true_intro.
-           split.
-           --- apply int64_eq_iff.
-               rewrite ! Byte.unsigned_repr; [| unfold Byte.max_unsigned; simpl; lia].
-               rewrite ! Int.unsigned_repr; [| unfold Int.max_unsigned; simpl; lia].
-               Search Int64.bitfield_insert.
-               bsolver. 
-               rewrite Z.eqb_neq in *.
-               admit.
-           --- destruct l as [| h0 l0]; [rewrite Coqlib.nth_error_nil in Hnth; inversion Hnth |].
-               destruct (nth_error l0 pc) eqn:Hnth2. ---- apply andb_true_intro. split. apply int64_eq_iff.
 
 
 
-Admitted.
-    
+
+
+
+
